lib/grammarMLScript.sml
@@ -1,0 +1,66 @@
+open HolKernel Parse boolLib bossLib
+
+open setLemmasTheory containerLemmasTheory
+open symbolDefTheory grammarDefTheory
+
+val _ = new_theory "grammarML"
+
+val nonTerminals = nonTerminals_def
+val terminals = terminals_def
+val rule_nonterminals = rule_nonterminals_def
+val rule_terminals = rule_terminals_def
+val allSyms = allSyms_def
+
+val nonTerminalsML =  Define
+`(nonTerminalsML (G [] s) = {NTS s}) ∧
+ (nonTerminalsML (G (rule l r::rs) s) =
+      set (FILTER isNonTmnlSym (NTS l :: r)) ∪
+      nonTerminalsML (G rs s))`;
+
+
+val terminalsML = Define
+`(terminalsML (G [] s) = LIST_TO_SET []) ∧
+ (terminalsML (G (rule l r::rs) s) =
+      LIST_TO_SET (FILTER isTmnlSym r) ∪ terminalsML (G rs s))`;
+
+val nonTerminalsEq = store_thm
+("nonTerminalsEq",
+``nonTerminals g = nonTerminalsML g``,
+Cases_on `g` THEN
+Induct_on `l` THEN
+SRW_TAC [] [nonTerminals, nonTerminalsML] THEN
+Cases_on `h` THEN
+FULL_SIMP_TAC (srw_ss()) [rule_nonterminals,nonTerminalsML,
+			  isNonTmnlSym_def,nonTerminals] THEN
+`nonTerminalsML (G l n) =
+     NTS n INSERT BIGUNION (IMAGE rule_nonterminals (set l))`
+	 by SRW_TAC [] [] THEN
+ONCE_ASM_REWRITE_TAC [] THEN
+SRW_TAC [] [filter_seteq,insert_union,isNonTmnlSym_def]);
+
+
+val terminalsEq = store_thm
+("terminalsEq",
+``terminals g = terminalsML g``,
+Cases_on `g` THEN
+Induct_on `l` THEN
+SRW_TAC [] [terminals, terminalsML] THEN
+Cases_on `h` THEN
+FULL_SIMP_TAC (srw_ss()) [terminalsML,isTmnlSym_def,terminals,
+			  rule_terminals] THEN
+`terminalsML (G l n) = BIGUNION (IMAGE rule_terminals (set l))`
+				by SRW_TAC [] [] THEN
+ONCE_ASM_REWRITE_TAC [] THEN
+FULL_SIMP_TAC (srw_ss()) [filter_seteq,insert_union,
+			  isTmnlSym_def]);
+
+val allSymsML = Define
+`allSymsML g = nonTerminalsML g ∪ terminalsML g`;
+
+
+val allSymsEq = store_thm (
+"allSymsEq",
+``allSyms g = allSymsML g``,
+SRW_TAC [][allSyms, allSymsML, terminalsEq, nonTerminalsEq]);
+
+val _ = export_theory()
